{
 "cells": [
  {
   "cell_type": "markdown",
   "metadata": {},
   "source": [
    "# Project 2"
   ]
  },
  {
   "cell_type": "markdown",
   "metadata": {},
   "source": [
    "# Task 1\n",
    "\n",
    "\n",
    "c) We have the following spaces\n",
    "\n",
    "$$\n",
    "\\tau_n :=  \\{ f \\mid f(x) = \\sum_{k = -n}^n c_k e^{2 {\\pi i k x}}, c_{-n}, c_{-n+1}, ..., c_n \\in \\mathbb{C} \\}\n",
    "$$\n",
    "and\n",
    "$$\n",
    "S_n := \\{ f \\mid f(x) = \\frac{a_0}{2} + \\sum_{k = i}^n a_k\\cos(2 \\pi kx) + b_k \\sin(2 \\pi kx), a_0,a_1...,a_n, b_1,...,b_n \\in \\mathbb{R}\\}\n",
    "$$\n",
    "\n",
    "\n",
    "We want to use the results from __a)__ and __b)__ to find orthonormal bases for these spaces. \n",
    "\n",
    "Because \n",
    "\n",
    "\n",
    "We want to show by __Eulers identity__ that $\\tau_n = S_n$.\n",
    "\n",
    "For an $f \\in \\tau_n $ we have that\n",
    "\n",
    "$$\n",
    "f(x) = \\sum_{k = -n}^n c_k e^{2\\pi ik x} = \\sum_{k = 1}^n c_{-k} e^{-2 \\pi ikx} +  \\sum_{k = 1}^n c_{k} e^{2 \\pi ikx} + c_0\n",
    "$$\n",
    "\n",
    "From Eulers identity we have\n",
    "\n",
    "$$\n",
    "e^{ix} = \\cos(x) + i\\sin(x)\n",
    "$$\n",
    "\n",
    "Such that\n",
    "\n",
    "$$\n",
    "\\begin{align}\n",
    "c_0 + \\sum_{k = 1}^n c_{-k} e^{-2 \\pi ikx} +  \\sum_{k = 1}^n c_{k} e^{2 \\pi ikx}  &= c_0 +\\sum_{k = 1}^n c_{-k} (\\cos(-2 \\pi kx)+ i \\sin(-2 \\pi kx))+\\sum_{k = 1}^n c_{k} (\\cos(2 \\pi kx)+ i \\sin(2 \\pi kx))\n",
    "\\\\\n",
    "&= c_0 + \\sum_{k = 1}^n(c_{-k} + c_k)\\cos(2 \\pi kx)+ i(c_k - c_{-k})\\sin(2 \\pi kx)\n",
    "\\end{align}\n",
    "$$\n",
    "\n",
    "Let now $a_k = c_{-k} + c_k$. Because $c_k = \\bar c_{-k}$, we have that $a_k = c_{-k} + c_k$ must be $2 Re(c_k)$ and must therefore fulfill $a_k \\in \\mathbb{R}$ such that $a_0 = 2c_0, \\implies c_0 = \\frac{a_0}{2}$. Let further $b_k = i(c_k - c_{-k})$. Because $c_k - c_{-k} = 2Im(c_k)$, $b_k = i(c_k - c_{-k})$ must be a real number such that $b_k \\in \\mathbb{R}$. We thus have that\n",
    "\n",
    "$$\n",
    "f(x) = \\sum_{k = -n}^n c_k e^{2\\pi ik x}  = c_0 + \\sum_{k = 1}^n(c_{-k} + c_k)\\cos(2 \\pi kx)+ i(c_k - c_{-k})\\sin(2 \\pi kx) = \\frac{a_0}{2} + \\sum_{k = 1}^n a_k \\cos(2 \\pi kx) + b_k \\sin(2 \\pi kx)\n",
    "$$"
   ]
  },
  {
   "cell_type": "markdown",
   "metadata": {},
   "source": [
    "Because $a_k, b_k \\in \\mathbb{R}$, we observe that the element $f \\in \\tau_n$ is equal to the same element $f \\in S_n$. Thus $\\tau_n = S_n$. $\\square$\n",
    "\n",
    "We have from a) that $<e^{2 \\pi ik \\cdot},e^{2 \\pi ih\\cdot}>=0$ when $k \\ne h$. \n",
    "\n",
    "Because $\\tau_n$ consists of $2n +1$ linearly independent vectors, the dimension of $\\tau_n$, $\\dim\\tau_n$, must be $2n+1$. Thus we have $\\dim\\tau_n = 2n +1$."
   ]
  },
  {
   "cell_type": "markdown",
   "metadata": {},
   "source": [
    "d)\n",
    "\n",
    "We now want to use the representation of $S_n := \\{ f \\mid f(x) = \\frac{a_0}{2} + \\sum_{k = i}^n a_k\\cos(2 \\pi kx) + b_k \\sin(2 \\pi kx), a_0,a_1...,a_n, b_1,...,b_n \\in \\mathbb{R}\\}$ to prove that the Fourier coefficients $a_0,a_1,...,a_n, b_1,....,b_n$ of a function $f \\in S_n$ can be computed as\n",
    "\n",
    "$$\n",
    "a_k = 2\\int_{-\\frac{1}{2}}^{\\frac{1}{2}}f(x) \\cos(2 \\pi kx) dx\n",
    "$$\n",
    "\n",
    "and\n",
    "$$\n",
    "b_k = 2\\int_{-\\frac{1}{2}}^{\\frac{1}{2}}f(x) \\sin(2 \\pi kx) dx\n",
    "$$\n",
    "\n",
    "Let $X = [x_0, x_0 + T]$ and let $T = 1$ be the period. We have for an $f \\in S_n$ that \n",
    "\n",
    "$$\n",
    "f(x) = \\frac{a_0}{2} + \\sum_{k = i}^n a_k\\cos(2 \\pi kx) + b_k \\sin(2 \\pi kx)\n",
    "$$\n",
    "\n",
    "Which can be written as\n",
    "\n",
    "$$\n",
    "f(x) = \\frac{a_0}{2} + a_1\\cos(2 \\pi x) + a_2\\cos(4 \\pi x) + ... +a_k\\cos(2 \\pi k x) + .. + b_1\\sin(2 \\pi x) + .. + b_k\\sin(2 \\pi kx)\n",
    "$$\n",
    "\n",
    "We start by deriving $a_0$. Taking the integral of both sides over one period we obtain\n",
    "\n",
    "$$\n",
    "\\int_X f(x) dx = \\int_X \\frac{a_0}{2} dx + \\int_X a_1\\cos(2 \\pi x) dx+ \\int_Xa_2\\cos(4 \\pi x) dx + ... +\\int_X a_k\\cos(2 \\pi k x) dx+ .. + \\int_X b_1\\sin(2 \\pi x) dx + .. + \\int_X b_k\\sin(2 \\pi kx)dx\n",
    "$$\n",
    "\n",
    "For $X = [x_0, x_0 + T]$. Because the integrals of a sine or cosine over one period is zero, all the integrals of the right hand side equals zero, and thus we are left with\n",
    "\n",
    "$$\n",
    "\\int_X f(x) dx = \\int_X \\frac{a_0}{2} dx  \\implies a_0 = \\frac{2}{T}\\int_X f(x) dx = \\frac{2}{T}\\int_X f(x) dx = \\frac{2}{T}\\int_{x_0}^{x_0 + T} f(x) dx\n",
    "$$\n",
    "\n",
    "For $x_0 = \\frac{1}{2}$ and $T = 1$ we obtain\n",
    "\n",
    "$$\n",
    "a_0 = \\frac{2}{T}\\int_{x_0}^{x_0 + T} f(x) dx = 2 \\int_{-\\frac{1}{2}}^{\\frac{1}{2}} f(x) dx\n",
    "$$\n",
    "\n",
    "Going back to the original expression we now want to find $a_k$. By multiplying by $\\cos(2 \\pi kx)$ we obtain\n",
    "\n",
    "$$\n",
    "f(x)\\cos(2 \\pi kx) = \\frac{a_0}{2}\\cos(2 \\pi kx) + a_1\\cos(2 \\pi x)\\cos(2 \\pi kx) + a_2\\cos(4 \\pi x)\\cos(2 \\pi kx) + ... +a_k\\cos(2 \\pi k x)\\cos(2 \\pi kx) + .. + b_1\\sin(2 \\pi x)\\cos(2 \\pi kx) + .. + b_k\\sin(2 \\pi kx)\\cos(2 \\pi kx)\n",
    "$$\n",
    "\n",
    "Taking the integral of both sides over one period we obtain\n",
    "\n",
    "$$\n",
    "\\int_X f(x)\\cos(2 \\pi kx) dx = \\int_X  \\frac{a_0}{2}\\cos(2 \\pi kx) dx+\\int_X a_1\\cos(2 \\pi x)\\cos(2 \\pi kx) dx + \\int_X a_2\\cos(4 \\pi x)\\cos(2 \\pi kx) dx + ... + \\int_X  a_k\\cos(2 \\pi k x)\\cos(2 \\pi kx) dx + .. + \\int_X  b_1\\sin(2 \\pi x)\\cos(2 \\pi kx) dx + .. + \\int_X  b_k\\sin(2 \\pi kx)\\cos(2 \\pi kx) dx\n",
    "$$\n",
    "\n",
    "Using that all cosine integrals over one period evaluates to zero, and using the following statements\n",
    "\n",
    "$$\n",
    "\\int_X \\sin(nx) \\cos(kx) dx = 0 \n",
    "$$\n",
    "\n",
    "$$\n",
    "\\int_X \\cos(nx) \\cos(kx) dx = 0  \\ Â (n \\ne k)\n",
    "$$\n",
    "\n",
    "$$\n",
    "\\int_X \\sin(nx) \\sin(kx) dx = 0  \\  (n \\ne k)\n",
    "$$\n",
    "\n",
    "We then observe that the expression we are left with is given by\n",
    "\n",
    "$$\n",
    "\\int_X f(x)\\cos(2 \\pi kx) dx  = \\int_X a_k \\cos^2(2 \\pi kx) dx = a_k \\frac{T}{2}\n",
    "$$\n",
    "\n",
    "Thus $a_k$ is given by\n",
    "\n",
    "$$\n",
    "a_k = \\frac{2}{T}\\int_X f(x) \\cos(2 \\pi kx) dx\n",
    "$$\n",
    "\n",
    "Which for our values is given by\n",
    "$$\n",
    "a_k = 2\\int_{-\\frac{1}{2}}^{\\frac{1}{2}} f(x) \\cos(2 \\pi kx) dx\n",
    "$$\n",
    "\n",
    "What remains is to find an expression for $b_k$. The procedure is similar as for $a_k$, but now we start by multiplying by $\\sin(2 \\pi kx) $\n",
    "\n",
    "$$\n",
    "f(x)\\sin(2 \\pi kx) = \\frac{a_0}{2}\\sin(2 \\pi kx) + a_1\\cos(2 \\pi x)\\sin(2 \\pi kx) + a_2\\cos(4 \\pi x)\\sin(2 \\pi kx) + ... +a_k\\cos(2 \\pi k x)\\sin(2 \\pi kx) + .. + b_1\\sin(2 \\pi x)\\sin(2 \\pi kx) + .. + b_k\\sin(2 \\pi kx)\\sin(2 \\pi kx)\n",
    "$$\n",
    "\n",
    "Taking the integral of both sides over one period we obtain\n",
    "\n",
    "$$\n",
    "\\int_X f(x)\\sin(2 \\pi kx) dx = \\int_X  \\frac{a_0}{2}\\sin(2 \\pi kx) dx+\\int_X a_1\\cos(2 \\pi x)\\sin(2 \\pi kx) dx + \\int_X a_2\\cos(4 \\pi x)\\sin(2 \\pi kx) dx + ... + \\int_X  a_k\\cos(2 \\pi k x)\\sin(2 \\pi kx) dx + .. + \\int_X  b_1\\sin(2 \\pi x)\\sin(2 \\pi kx) dx + .. + \\int_X  b_k\\sin(2 \\pi kx)\\sin(2 \\pi kx) dx\n",
    "$$\n",
    "\n",
    "By the same arguments and reasoning as for $a_k$, we see that we now are left with the following expression\n",
    "\n",
    "$$\n",
    "\\int_X f(x) \\sin(2 \\pi kx) dx = \\int_X b_k \\sin^2(2 \\pi kx) dx = b_k \\frac{T}{2}\n",
    "$$\n",
    "\n",
    "And thus $b_k$ is given by\n",
    "\n",
    "$$\n",
    "b_k = \\frac{2}{T}\\int_X  f(x) \\sin(2 \\pi kx) dx = \\frac{2}{T}\\int_{-\\frac{1}{2}}^{\\frac{1}{2}} f(x) \\sin(2 \\pi kx) dx\n",
    "$$\n",
    "\n",
    "And we have thus derived the Fourier coefficients. $\\square$"
   ]
  },
  {
   "cell_type": "markdown",
   "metadata": {},
   "source": [
    "# Task 2\n",
    "\n",
    "### b)\n",
    "We want to prove that for any $k$ it holds\n",
    "$$c_{k}(\\tau_{N}f)=e^{-2\\pi ik/N}c_k(f)$$\n",
    "Where $\\tau_{N}(f)=f(\\cdot- \\frac{1}{N})$\n",
    "$$c_{k}(\\tau_{N}(f))= \\frac{1}{N}\\sum\\limits_{j=0}^{N-1}f\\left(x_{j}- \\frac{1}{N}\\right)e^{-2\\pi ijk/N}$$\n",
    "$$=\\frac{1}{N}\\sum\\limits_{j=0}^{N-1}f\\left(\\frac{j}{N}- \\frac{1}{N}\\right)e^{-2\\pi ijk/N}$$\n",
    "$$\\begin{align*}\n",
    "&=\\frac{1}{N}\\sum\\limits_{j=0}^{N-1}f_{j-1}e^{-2\\pi ijk/N}\\\\\n",
    "&= \\frac{1}{N}\\left(f_{-1}+\\sum\\limits_{j=0}^{N-2}f_{j}e^{-2\\pi i(j+1)k/N}\\right)\\\\\n",
    "\\end{align*}$$\n",
    "Since by periodicity $f_{-1}=f_{N-1}$ and $e^{-2\\pi iNk/N}=1$ ($k\\in\\mathbb{Z}$), we can put this back in the sum:\n",
    "$$c_{k}(\\tau_{N} f)=\\frac{1}{N}\\sum\\limits_{j=0}^{N-1}f_{j}e^{-2\\pi i(j+1)k/N}$$\n",
    "$$=e^{-2\\pi ik/N}\\frac{1}{N}\\sum\\limits_{j=0}^{N-1}f_{j}e^{-2\\pi ijk/N}$$\n",
    "$$c_{k}(\\tau_{N}f)=e^{-2\\pi ik/N}c_{k}(f)\\qquad\\square$$"
   ]
  },
  {
   "cell_type": "markdown",
   "metadata": {},
   "source": [
    "## Task 3\n",
    "\n",
    "a) We have the so-called __Dirichlet kernel__ given by\n",
    "$$\n",
    "D_n(x) = \\frac{1}{2n+1}\\sum_{k = -n}^n e^{2 \\pi i kx}\n",
    "$$\n",
    "\n",
    "For $n \\in \\mathbf{N}_0$"
   ]
  }
 ],
 "metadata": {
  "kernelspec": {
   "display_name": "Python 3.9.12 64-bit",
   "language": "python",
   "name": "python3"
  },
  "language_info": {
   "name": "python",
   "version": "3.9.12"
  },
  "orig_nbformat": 4,
  "vscode": {
   "interpreter": {
    "hash": "b0fa6594d8f4cbf19f97940f81e996739fb7646882a419484c72d19e05852a7e"
   }
  }
 },
 "nbformat": 4,
 "nbformat_minor": 2
}
